trillium/program_logic/ectx_lifting.v
@@ -28,7 +28,7 @@ Lemma wp_lift_head_step_fupd {s E Φ} e1 ζ:
     ∀ e2 σ2 efs, ⌜head_step e1 σ1 e2 σ2 efs⌝ ={∅}=∗ ▷ |={∅,E}=>
       ∃ δ2 ℓ,
         state_interp
-          (trace_extend extr (Some ζ) (tp1 ++ fill K e2 :: tp2 ++ efs, σ2))
+          (trace_extend extr (inl ζ) (tp1 ++ fill K e2 :: tp2 ++ efs, σ2))
           (trace_extend atr ℓ δ2) ∗
       WP e2 @ s; ζ; E {{ Φ }} ∗
       [∗ list] i ↦ef ∈ efs, WP ef @ s; locale_of (tp1 ++ ectx_fill K e1 :: tp2 ++ (take i efs)) ef; ⊤
@@ -54,7 +54,7 @@ Lemma wp_lift_head_step {s E Φ} e1 ζ:
     ▷ ∀ e2 σ2 efs, ⌜head_step e1 σ1 e2 σ2 efs⌝ ={∅,E}=∗
       ∃ δ2 ℓ, 
         state_interp
-          (trace_extend extr (Some ζ) (tp1 ++ fill K e2 :: tp2 ++ efs, σ2))
+          (trace_extend extr (inl ζ) (tp1 ++ fill K e2 :: tp2 ++ efs, σ2))
           (trace_extend atr ℓ δ2) ∗
       WP e2 @ s; ζ; E {{ Φ }} ∗
       [∗ list] i ↦ef ∈ efs, WP ef @ s; locale_of (tp1 ++ ectx_fill K e1 :: tp2 ++ (take i efs)) ef; ⊤
@@ -102,7 +102,7 @@ Lemma wp_lift_atomic_head_step_fupd {s E1 E2 Φ} e1 ζ:
     ∀ e2 σ2 efs, ⌜head_step e1 σ1 e2 σ2 efs⌝ ={E1}[E2]▷=∗
       ∃ δ2 ℓ,
         state_interp
-          (trace_extend extr (Some ζ) (tp1 ++ fill K e2 :: tp2 ++ efs, σ2))
+          (trace_extend extr (inl ζ) (tp1 ++ fill K e2 :: tp2 ++ efs, σ2))
           (trace_extend atr ℓ δ2) ∗
       from_option Φ False (to_val e2) ∗
       [∗ list] i ↦ef ∈ efs, WP ef @ s; locale_of (tp1 ++ ectx_fill K e1 :: tp2 ++ (take i efs)) ef; ⊤
@@ -128,7 +128,7 @@ Lemma wp_lift_atomic_head_step {s E Φ} e1 ζ:
     ▷ ∀ e2 σ2 efs, ⌜head_step e1 σ1 e2 σ2 efs⌝ ={E}=∗
       ∃ δ2 ℓ, 
         state_interp
-          (trace_extend extr (Some ζ) (tp1 ++ fill K e2 :: tp2 ++ efs, σ2))
+          (trace_extend extr (inl ζ) (tp1 ++ fill K e2 :: tp2 ++ efs, σ2))
           (trace_extend atr ℓ δ2) ∗
       from_option Φ False (to_val e2) ∗
       [∗ list] i ↦ef ∈ efs, WP ef @ s; locale_of (tp1 ++ ectx_fill K e1 :: tp2 ++ (take i efs)) ef; ⊤
@@ -154,7 +154,7 @@ Lemma wp_lift_atomic_head_step_no_fork_fupd {s E1 E2 Φ} e1 ζ:
       ∃ δ2 ℓ,
         ⌜efs = [] ⌝∗
         state_interp
-          (trace_extend extr (Some ζ) (tp1 ++ fill K e2 :: tp2 ++ efs, σ2))
+          (trace_extend extr (inl ζ) (tp1 ++ fill K e2 :: tp2 ++ efs, σ2))
           (trace_extend atr ℓ δ2) ∗
       from_option Φ False (to_val e2))
   ⊢ WP e1 @ s; ζ; E1 {{ Φ }}.
@@ -181,7 +181,7 @@ Lemma wp_lift_atomic_head_step_no_fork {s E Φ} e1 ζ:
     ▷ ∀ e2 σ2 efs, ⌜head_step e1 σ1 e2 σ2 efs⌝ ={E}=∗
        ∃ δ2 ℓ, 
          ⌜efs = []⌝ ∗ state_interp
-          (trace_extend extr (Some ζ) (tp1 ++ fill K e2 :: tp2 ++ efs, σ2))
+          (trace_extend extr (inl ζ) (tp1 ++ fill K e2 :: tp2 ++ efs, σ2))
           (trace_extend atr ℓ δ2) ∗
       from_option Φ False (to_val e2))
   ⊢ WP e1 @ s; ζ; E {{ Φ }}.
